tll

coq/sta_conf.v
@@ -39,6 +39,74 @@ Inductive pstep : term -> term -> Prop :=
   pstep m m' ->
   pstep n n' ->
   pstep (App (Lam1 A m s) n) (m'.[n'/])
+| pstep_sig0 A A' B B' s :
+  pstep A A' ->
+  pstep B B' ->
+  pstep (Sig0 A B s) (Sig0 A' B' s)
+| pstep_sig1 A A' B B' s :
+  pstep A A' ->
+  pstep B B' ->
+  pstep (Sig1 A B s) (Sig1 A' B' s)
+| pstep_pair0 m m' n n' s :
+  pstep m m' ->
+  pstep n n' ->
+  pstep (Pair0 m n s) (Pair0 m' n' s)
+| pstep_pair1 m m' n n' s :
+  pstep m m' ->
+  pstep n n' ->
+  pstep (Pair1 m n s) (Pair1 m' n' s)
+| pstep_letin A A' m m' n n' :
+  pstep A A' ->
+  pstep m m' ->
+  pstep n n' ->
+  pstep (LetIn A m n) (LetIn A' m' n')
+| pstep_iota0 A m1 m1' m2 m2' n n' s :
+  pstep m1 m1' ->
+  pstep m2 m2' ->
+  pstep n n' ->
+  pstep (LetIn A (Pair0 m1 m2 s) n) (n'.[m2',m1'/])
+| pstep_iota1 A m1 m1' m2 m2' n n' s :
+  pstep m1 m1' ->
+  pstep m2 m2' ->
+  pstep n n' ->
+  pstep (LetIn A (Pair1 m1 m2 s) n) (n'.[m2',m1'/])
+| pstep_with A A' B B' s :
+  pstep A A' ->
+  pstep B B' ->
+  pstep (With A B s) (With A' B' s)
+| pstep_apair m m' n n' s :
+  pstep m m' ->
+  pstep n n' ->
+  pstep (APair m n s) (APair m' n' s)
+| pstep_fst m m' :
+  pstep m m' ->
+  pstep (Fst m) (Fst m')
+| pstep_snd m m' :
+  pstep m m' ->
+  pstep (Snd m) (Snd m')
+| pstep_proj1 m m' n s :
+  pstep m m' ->
+  pstep (Fst (APair m n s)) m'
+| pstep_proj2 m n n' s :
+  pstep n n' ->
+  pstep (Snd (APair m n s)) n'
+| pstep_id A A' m m' n n' :
+  pstep A A' ->
+  pstep m m' ->
+  pstep n n' ->
+  pstep (Id A m n) (Id A' m' n')
+| pstep_refl m m' :
+  pstep m m' ->
+  pstep (Refl m) (Refl m')
+| pstep_j A A' H H' P P' :
+  pstep A A' ->
+  pstep H H' ->
+  pstep P P' ->
+  pstep (J A H P) (J A' H' P')
+| pstep_jelim A H H' m m' :
+  pstep H H' ->
+  pstep m m' ->
+  pstep (J A H (Refl m)) H'.[m'/]
 | pstep_box : pstep Box Box.
 
 Definition sred σ τ := forall x : var, (σ x) ~>* (τ x).
@@ -48,10 +116,19 @@ Proof.
   move=> st. elim: st σ=>/={m n}; eauto using sta_step.
   { move=> A m n s σ.
     replace (m.[n/].[σ]) with (m.[up σ].[n.[σ]/]).
-    apply sta_beta0. autosubst. }
+    apply sta_step_beta0. autosubst. }
   { move=> A m n s σ.
     replace (m.[n/].[σ]) with (m.[up σ].[n.[σ]/]).
-    apply sta_beta1. autosubst. }
+    apply sta_step_beta1. autosubst. }
+  { move=>A m1 m2 n s σ.
+    replace (n.[m2,m1/].[σ]) with (n.[upn 2 σ].[m2.[σ],m1.[σ]/]).
+    apply: sta_step_iota0. autosubst. }
+  { move=>A m1 m2 n s σ.
+    replace (n.[m2,m1/].[σ]) with (n.[upn 2 σ].[m2.[σ],m1.[σ]/]).
+    apply: sta_step_iota1. autosubst. }
+  { move=>A H m σ.
+    replace (H.[m/].[σ]) with (H.[up σ].[m.[σ]/]).
+    apply: sta_step_jelim. autosubst. }
 Qed.
 
 Lemma sta_red_app m m' n n' :
@@ -59,8 +136,8 @@ Lemma sta_red_app m m' n n' :
 Proof.
   move=> r1 r2.
   apply: (star_trans (App m' n)).
-  apply: (star_hom (App^~ n)) r1=>x y. exact: sta_appL.
-  apply: star_hom r2. exact: sta_appR.
+  apply: (star_hom (App^~ n)) r1=>x y. exact: sta_step_appL.
+  apply: star_hom r2. exact: sta_step_appR.
 Qed.
 
 Lemma sta_red_lam0 A A' m m' s :
@@ -68,8 +145,8 @@ Lemma sta_red_lam0 A A' m m' s :
 Proof.
   move=> r1 r2.
   apply: (star_trans (Lam0 A' m s)).
-  apply: (star_hom ((Lam0^~ m)^~ s)) r1=>x y. exact: sta_lam0L.
-  apply: (star_hom ((Lam0 A')^~ s)) r2=>x y. exact: sta_lam0R.
+  apply: (star_hom ((Lam0^~ m)^~ s)) r1=>x y. exact: sta_step_lam0L.
+  apply: (star_hom ((Lam0 A')^~ s)) r2=>x y. exact: sta_step_lam0R.
 Qed.
 
 Lemma sta_red_lam1 A A' m m' s :
@@ -77,8 +154,8 @@ Lemma sta_red_lam1 A A' m m' s :
 Proof.
   move=> r1 r2.
   apply: (star_trans (Lam1 A' m s)).
-  apply: (star_hom ((Lam1^~ m)^~ s)) r1=>x y. exact: sta_lam1L.
-  apply: (star_hom ((Lam1 A')^~ s)) r2=>x y. exact: sta_lam1R.
+  apply: (star_hom ((Lam1^~ m)^~ s)) r1=>x y. exact: sta_step_lam1L.
+  apply: (star_hom ((Lam1 A')^~ s)) r2=>x y. exact: sta_step_lam1R.
 Qed.
 
 Lemma sta_red_pi0 A A' B B' s :
@@ -86,8 +163,8 @@ Lemma sta_red_pi0 A A' B B' s :
 Proof.
   move=> r1 r2.
   apply: (star_trans (Pi0 A' B s)).
-  apply: (star_hom ((Pi0^~ B)^~ s)) r1=>x y. exact: sta_pi0L.
-  apply: (star_hom ((Pi0 A')^~ s)) r2=>x y. exact: sta_pi0R.
+  apply: (star_hom ((Pi0^~ B)^~ s)) r1=>x y. exact: sta_step_pi0L.
+  apply: (star_hom ((Pi0 A')^~ s)) r2=>x y. exact: sta_step_pi0R.
 Qed.
 
 Lemma sta_red_pi1 A A' B B' s :
@@ -95,8 +172,116 @@ Lemma sta_red_pi1 A A' B B' s :
 Proof.
   move=> r1 r2.
   apply: (star_trans (Pi1 A' B s)).
-  apply: (star_hom ((Pi1^~ B)^~ s)) r1=>x y. exact: sta_pi1L.
-  apply: (star_hom ((Pi1 A')^~ s)) r2=>x y. exact: sta_pi1R.
+  apply: (star_hom ((Pi1^~ B)^~ s)) r1=>x y. exact: sta_step_pi1L.
+  apply: (star_hom ((Pi1 A')^~ s)) r2=>x y. exact: sta_step_pi1R.
+Qed.
+
+Lemma sta_red_sig0 A A' B B' s :
+  A ~>* A' -> B ~>* B' -> Sig0 A B s ~>* Sig0 A' B' s.
+Proof.
+  move=> r1 r2.
+  apply: (star_trans (Sig0 A' B s)).
+  apply: (star_hom ((Sig0^~ B)^~ s)) r1=>x y. exact: sta_step_sig0L.
+  apply: (star_hom ((Sig0 A')^~ s)) r2=>x y. exact: sta_step_sig0R.
+Qed.
+
+Lemma sta_red_sig1 A A' B B' s :
+  A ~>* A' -> B ~>* B' -> Sig1 A B s ~>* Sig1 A' B' s.
+Proof.
+  move=> r1 r2.
+  apply: (star_trans (Sig1 A' B s)).
+  apply: (star_hom ((Sig1^~ B)^~ s)) r1=>x y. exact: sta_step_sig1L.
+  apply: (star_hom ((Sig1 A')^~ s)) r2=>x y. exact: sta_step_sig1R.
+Qed.
+
+Lemma sta_red_pair0 m m' n n' t :
+  m ~>* m' -> n ~>* n' -> Pair0 m n t ~>* Pair0 m' n' t.
+Proof.
+  move=>r1 r2.
+  apply: (star_trans (Pair0 m' n t)).
+  apply: (star_hom ((Pair0^~ n)^~ t)) r1=>x y. exact: sta_step_pair0L.
+  apply: (star_hom ((Pair0 m')^~ t)) r2=>x y. exact: sta_step_pair0R.
+Qed.
+
+Lemma sta_red_pair1 m m' n n' t :
+  m ~>* m' -> n ~>* n' -> Pair1 m n t ~>* Pair1 m' n' t.
+Proof.
+  move=>r1 r2.
+  apply: (star_trans (Pair1 m' n t)).
+  apply: (star_hom ((Pair1^~ n)^~ t)) r1=>x y. exact: sta_step_pair1L.
+  apply: (star_hom ((Pair1 m')^~ t)) r2=>x y. exact: sta_step_pair1R.
+Qed.
+
+Lemma sta_red_letin A A' m m' n n' :
+  A ~>* A' -> m ~>* m' -> n ~>* n' -> LetIn A m n ~>* LetIn A' m' n'.
+Proof.
+  move=>r1 r2 r3.
+  apply: (star_trans (LetIn A' m n)).
+  apply: (star_hom ((LetIn^~ m)^~ n)) r1=>x y. exact: sta_step_letinA.
+  apply: (star_trans (LetIn A' m' n)).
+  apply: (star_hom (LetIn A'^~ n)) r2=>x y. exact: sta_step_letinL.
+  apply: (star_hom (LetIn A' m')) r3=>x y. exact: sta_step_letinR.
+Qed.
+
+Lemma sta_red_with A A' B B' s :
+  A ~>* A' -> B ~>* B' -> With A B s ~>* With A' B' s.
+Proof.
+  move=>r1 r2.
+  apply: (star_trans (With A' B s)).
+  apply: (star_hom ((With^~ B)^~ s)) r1=>x y. exact: sta_step_withL.
+  apply: (star_hom ((With A')^~ s)) r2=>x y. exact: sta_step_withR.
+Qed.
+
+Lemma sta_red_apair m m' n n' s :
+  m ~>* m' -> n ~>* n' -> APair m n s ~>* APair m' n' s.
+Proof.
+  move=>r1 r2.
+  apply: (star_trans (APair m' n s)).
+  apply: (star_hom ((APair^~ n)^~ s)) r1=>x y. exact: sta_step_apairL.
+  apply: (star_hom ((APair m')^~ s)) r2=>x y. exact: sta_step_apairR.
+Qed.
+
+Lemma sta_red_fst m m' :
+  m ~>* m' -> Fst m ~>* Fst m'.
+Proof.
+  move=>r.
+  apply: (star_hom Fst) r=>x y. exact: sta_step_fst.
+Qed.
+
+Lemma sta_red_snd m m' :
+  m ~>* m' -> Snd m ~>* Snd m'.
+Proof.
+  move=>r.
+  apply: (star_hom Snd) r=>x y. exact: sta_step_snd.
+Qed.
+
+Lemma sta_red_id A A' m m' n n' :
+  A ~>* A' -> m ~>* m' -> n ~>* n' -> Id A m n ~>* Id A' m' n'.
+Proof.
+  move=>r1 r2 r3.
+  apply: (star_trans (Id A' m n)).
+  apply: (star_hom ((Id^~ m)^~ n)) r1=>x y. exact: sta_step_idA.
+  apply: (star_trans (Id A' m' n)).
+  apply: (star_hom (Id A'^~ n)) r2=>x y. exact: sta_step_idL.
+  apply: (star_hom (Id A' m')) r3=>x y. exact: sta_step_idR.
+Qed.
+
+Lemma sta_red_refl m m' :
+  m ~>* m' -> Refl m ~>* Refl m'.
+Proof.
+  move=>r.
+  apply: (star_hom Refl) r=>x y. exact: sta_step_refl.
+Qed.
+
+Lemma sta_red_j A A' H H' P P' :
+  A ~>* A' -> H ~>* H' -> P ~>* P' -> J A H P ~>* J A' H' P'.
+Proof.
+  move=>r1 r2 r3.
+  apply: (star_trans (J A' H P)).
+  apply: (star_hom ((J^~ H)^~ P)) r1=>x y. exact: sta_step_jA.
+  apply: (star_trans (J A' H' P)).
+  apply: (star_hom (J A'^~P)) r2=>x y. exact: sta_step_jH.
+  apply: (star_hom (J A' H')) r3=>x y. exact: sta_step_jP.
 Qed.
 
 Lemma sta_red_subst m n σ : m ~>* n -> m.[σ] ~>* n.[σ].
@@ -125,10 +310,16 @@ Hint Resolve
   sta_red_app
   sta_red_lam0 sta_red_lam1
   sta_red_pi0 sta_red_pi1
+  sta_red_sig0 sta_red_sig1
+  sta_red_pair0 sta_red_pair1
+  sta_red_letin
+  sta_red_with sta_red_apair
+  sta_red_fst sta_red_snd
+  sta_red_id sta_red_refl sta_red_j
   sred_up sred_upn : sta_red_congr.
 
 Lemma sta_red_compat σ τ s : sred σ τ -> sta_red s.[σ] s.[τ].
-Proof. elim: s σ τ => *; asimpl; eauto with sta_red_congr. Qed.
+Proof. elim: s σ τ => *; asimpl; eauto 9 with sta_red_congr. Qed.
 
 Definition sconv (σ τ : var -> term) := forall x, σ x === τ x.
 
@@ -137,8 +328,8 @@ Lemma sta_conv_app m m' n n' :
 Proof.
   move=> r1 r2.
   apply: (conv_trans (App m' n)).
-  apply: (conv_hom (App^~ n)) r1=>x y. exact: sta_appL.
-  apply: conv_hom r2. exact: sta_appR.
+  apply: (conv_hom (App^~ n)) r1=>x y. exact: sta_step_appL.
+  apply: conv_hom r2. exact: sta_step_appR.
 Qed.
 
 Lemma sta_conv_lam0 A A' m m' s :
@@ -146,8 +337,8 @@ Lemma sta_conv_lam0 A A' m m' s :
 Proof.
   move=> r1 r2.
   apply: (conv_trans (Lam0 A' m s)).
-  apply: (conv_hom ((Lam0^~ m)^~ s)) r1=>x y. exact: sta_lam0L.
-  apply: (conv_hom ((Lam0 A')^~ s)) r2=>x y. exact: sta_lam0R.
+  apply: (conv_hom ((Lam0^~ m)^~ s)) r1=>x y. exact: sta_step_lam0L.
+  apply: (conv_hom ((Lam0 A')^~ s)) r2=>x y. exact: sta_step_lam0R.
 Qed.
 
 Lemma sta_conv_lam1 A A' m m' s :
@@ -155,8 +346,8 @@ Lemma sta_conv_lam1 A A' m m' s :
 Proof.
   move=> r1 r2.
   apply: (conv_trans (Lam1 A' m s)).
-  apply: (conv_hom ((Lam1^~ m)^~ s)) r1=>x y. exact: sta_lam1L.
-  apply: (conv_hom ((Lam1 A')^~ s)) r2=>x y. exact: sta_lam1R.
+  apply: (conv_hom ((Lam1^~ m)^~ s)) r1=>x y. exact: sta_step_lam1L.
+  apply: (conv_hom ((Lam1 A')^~ s)) r2=>x y. exact: sta_step_lam1R.
 Qed.
 
 Lemma sta_conv_pi0 A A' B B' s :
@@ -164,8 +355,8 @@ Lemma sta_conv_pi0 A A' B B' s :
 Proof.
   move=> r1 r2.
   apply: (conv_trans (Pi0 A' B s)).
-  apply: (conv_hom ((Pi0^~ B)^~ s)) r1=>x y. exact: sta_pi0L.
-  apply: (conv_hom ((Pi0 A')^~ s)) r2=>x y. exact: sta_pi0R.
+  apply: (conv_hom ((Pi0^~ B)^~ s)) r1=>x y. exact: sta_step_pi0L.
+  apply: (conv_hom ((Pi0 A')^~ s)) r2=>x y. exact: sta_step_pi0R.
 Qed.
 
 Lemma sta_conv_pi1 A A' B B' s :
@@ -173,8 +364,116 @@ Lemma sta_conv_pi1 A A' B B' s :
 Proof.
   move=> r1 r2.
   apply: (conv_trans (Pi1 A' B s)).
-  apply: (conv_hom ((Pi1^~ B)^~ s)) r1=>x y. exact: sta_pi1L.
-  apply: (conv_hom ((Pi1 A')^~ s)) r2=>x y. exact: sta_pi1R.
+  apply: (conv_hom ((Pi1^~ B)^~ s)) r1=>x y. exact: sta_step_pi1L.
+  apply: (conv_hom ((Pi1 A')^~ s)) r2=>x y. exact: sta_step_pi1R.
+Qed.
+
+Lemma sta_conv_sig0 A A' B B' s :
+  A === A' -> B === B' -> Sig0 A B s === Sig0 A' B' s.
+Proof.
+  move=> r1 r2.
+  apply: (conv_trans (Sig0 A' B s)).
+  apply: (conv_hom ((Sig0^~ B)^~ s)) r1=>x y. exact: sta_step_sig0L.
+  apply: (conv_hom ((Sig0 A')^~ s)) r2=>x y. exact: sta_step_sig0R.
+Qed.
+
+Lemma sta_conv_sig1 A A' B B' s :
+  A === A' -> B === B' -> Sig1 A B s === Sig1 A' B' s.
+Proof.
+  move=> r1 r2.
+  apply: (conv_trans (Sig1 A' B s)).
+  apply: (conv_hom ((Sig1^~ B)^~ s)) r1=>x y. exact: sta_step_sig1L.
+  apply: (conv_hom ((Sig1 A')^~ s)) r2=>x y. exact: sta_step_sig1R.
+Qed.
+
+Lemma sta_conv_pair0 m m' n n' t :
+  m === m' -> n === n' -> Pair0 m n t === Pair0 m' n' t.
+Proof.
+  move=>r1 r2.
+  apply: (conv_trans (Pair0 m' n t)).
+  apply: (conv_hom ((Pair0^~ n)^~ t)) r1=>x y. exact: sta_step_pair0L.
+  apply: (conv_hom ((Pair0 m')^~ t)) r2=>x y. exact: sta_step_pair0R.
+Qed.
+
+Lemma sta_conv_pair1 m m' n n' t :
+  m === m' -> n === n' -> Pair1 m n t === Pair1 m' n' t.
+Proof.
+  move=>r1 r2.
+  apply: (conv_trans (Pair1 m' n t)).
+  apply: (conv_hom ((Pair1^~ n)^~ t)) r1=>x y. exact: sta_step_pair1L.
+  apply: (conv_hom ((Pair1 m')^~ t)) r2=>x y. exact: sta_step_pair1R.
+Qed.
+
+Lemma sta_conv_letin A A' m m' n n' :
+  A === A' -> m === m' -> n === n' -> LetIn A m n === LetIn A' m' n'.
+Proof.
+  move=>r1 r2 r3.
+  apply: (conv_trans (LetIn A' m n)).
+  apply: (conv_hom ((LetIn^~ m)^~ n)) r1=>x y. exact: sta_step_letinA.
+  apply: (conv_trans (LetIn A' m' n)).
+  apply: (conv_hom (LetIn A'^~ n)) r2=>x y. exact: sta_step_letinL.
+  apply: (conv_hom (LetIn A' m')) r3=>x y. exact: sta_step_letinR.
+Qed.
+
+Lemma sta_conv_with A A' B B' s :
+  A === A' -> B === B' -> With A B s === With A' B' s.
+Proof.
+  move=>r1 r2.
+  apply: (conv_trans (With A' B s)).
+  apply: (conv_hom ((With^~ B)^~ s)) r1=>x y. exact: sta_step_withL.
+  apply: (conv_hom ((With A')^~ s)) r2=>x y. exact: sta_step_withR.
+Qed.
+
+Lemma sta_conv_apair m m' n n' s :
+  m === m' -> n === n' -> APair m n s === APair m' n' s.
+Proof.
+  move=>r1 r2.
+  apply: (conv_trans (APair m' n s)).
+  apply: (conv_hom ((APair^~ n)^~ s)) r1=>x y. exact: sta_step_apairL.
+  apply: (conv_hom ((APair m')^~ s)) r2=>x y. exact: sta_step_apairR.
+Qed.
+
+Lemma sta_conv_fst m m' :
+  m === m' -> Fst m === Fst m'.
+Proof.
+  move=>r.
+  apply: (conv_hom Fst) r=>x y. exact: sta_step_fst.
+Qed.
+
+Lemma sta_conv_snd m m' :
+  m === m' -> Snd m === Snd m'.
+Proof.
+  move=>r.
+  apply: (conv_hom Snd) r=>x y. exact: sta_step_snd.
+Qed.
+
+Lemma sta_conv_id A A' m m' n n' :
+  A === A' -> m === m' -> n === n' -> Id A m n === Id A' m' n'.
+Proof.
+  move=>r1 r2 r3.
+  apply: (conv_trans (Id A' m n)).
+  apply: (conv_hom ((Id^~ m)^~ n)) r1=>x y. exact: sta_step_idA.
+  apply: (conv_trans (Id A' m' n)).
+  apply: (conv_hom (Id A'^~ n)) r2=>x y. exact: sta_step_idL.
+  apply: (conv_hom (Id A' m')) r3=>x y. exact: sta_step_idR.
+Qed.
+
+Lemma sta_conv_refl m m' :
+  m === m' -> Refl m === Refl m'.
+Proof.
+  move=>r.
+  apply: (conv_hom Refl) r=>x y. exact: sta_step_refl.
+Qed.
+
+Lemma sta_conv_j A A' H H' P P' :
+  A === A' -> H === H' -> P === P' -> J A H P === J A' H' P'.
+Proof.
+  move=>r1 r2 r3.
+  apply: (conv_trans (J A' H P)).
+  apply: (conv_hom ((J^~ H)^~ P)) r1=>x y. exact: sta_step_jA.
+  apply: (conv_trans (J A' H' P)).
+  apply: (conv_hom (J A'^~ P)) r2=>x y. exact: sta_step_jH.
+  apply: (conv_hom (J A' H')) r3=>x y. exact: sta_step_jP.
 Qed.
 
 Lemma sta_conv_subst σ m n :
@@ -199,37 +498,59 @@ Hint Resolve
   sta_conv_app
   sta_conv_lam0 sta_conv_lam1
   sta_conv_pi0 sta_conv_pi1
+  sta_conv_sig0 sta_conv_sig1
+  sta_conv_pair0 sta_conv_pair1
+  sta_conv_letin
+  sta_conv_with sta_conv_apair
+  sta_conv_fst sta_conv_snd
+  sta_conv_id sta_conv_refl sta_conv_j
   sconv_up sconv_upn : sta_conv_congr.
 
 Lemma sta_conv_compat σ τ s :
   sconv σ τ -> s.[σ] === s.[τ].
-Proof. elim: s σ τ => *; asimpl; eauto with sta_conv_congr. Qed.
+Proof. elim: s σ τ => *; asimpl; eauto 9 with sta_conv_congr. Qed.
 
 Lemma sta_conv_beta m n1 n2 : n1 === n2 -> m.[n1/] === m.[n2/].
 Proof. move=> c. by apply: sta_conv_compat => -[]. Qed.
 
-Lemma pstep_refl m : pstep m m.
+Lemma pstep_reflexive m : pstep m m.
 Proof. elim: m; eauto using pstep. Qed.
-Hint Resolve pstep_refl.
+Hint Resolve pstep_reflexive.
 
 Lemma sta_step_pstep m m' : sta_step m m' -> pstep m m'.
-Proof with eauto using pstep, pstep_refl. elim... Qed.
+Proof with eauto using pstep, pstep_reflexive. elim... Qed.
 
 Lemma pstep_sta_red m n : pstep m n -> m ~>* n.
-Proof.
+Proof with eauto.
   elim=>{m n}//=; eauto with sta_red_congr.
   { move=> A m m' n n' s p1 r1 p2 r2.
     apply: starES. by constructor.
-    apply: (star_trans (m'.[n.:Var])). exact: sta_red_subst.
-    by apply: sta_red_compat => -[|]. }
+    apply: (star_trans (m'.[n/])). exact: sta_red_subst.
+    by apply: sta_red_compat=>-[|]. }
   { move=> A m m' n n' s p1 r1 p2 r2.
     apply: starES. by constructor.
-    apply: (star_trans (m'.[n.:Var])). exact: sta_red_subst.
-    by apply: sta_red_compat => -[|]. }
+    apply: (star_trans (m'.[n/])). exact: sta_red_subst.
+    by apply: sta_red_compat=>-[|]. }
+  { move=> A m1 m1' m2 m2' n n' s p1 r1 p2 r2 p r.
+    apply: starES. by constructor.
+    apply: (star_trans (n'.[m2,m1/])). exact: sta_red_subst.
+    by apply: sta_red_compat=>-[|-[]]. }
+  { move=> A m1 m1' m2 m2' n n' s p1 r1 p2 r2 p r.
+    apply: starES. by constructor.
+    apply: (star_trans (n'.[m2,m1/])). exact: sta_red_subst.
+    by apply: sta_red_compat=>-[|-[]]. }
+  { move=>m m' n s p r.
+    apply: starES. by constructor. eauto. }
+  { move=>m m' n s p r.
+    apply: starES. by constructor. eauto. }
+  { move=>A H H' m m' p1 r1 p2 r2.
+    apply: starES. by constructor.
+    apply: (star_trans H'.[m/]). exact: sta_red_subst.
+    by apply: sta_red_compat=>-[|-[]]. }
 Qed.
 
 Lemma pstep_subst m n σ : pstep m n -> pstep m.[σ] n.[σ].
-Proof with eauto using pstep, pstep_refl.
+Proof with eauto using pstep, pstep_reflexive.
   move=>ps. elim: ps σ=>{m n}...
   { move=>A m m' n n' s ps1 ih1 ps2 ih2 σ.
     asimpl.
@@ -239,15 +560,27 @@ Proof with eauto using pstep, pstep_refl.
     asimpl.
     pose proof (pstep_beta1 A.[σ] s (ih1 (up σ)) (ih2 σ)) as H.
     by asimpl in H. }
+  { move=>A m1 m1' m2 m2' n n' s pm1 ihm1 pm2 ihm2 pn ihn σ.
+    asimpl.
+    pose proof (pstep_iota0 A.[up σ] s (ihm1 σ) (ihm2 σ) (ihn (upn 2 σ))).
+    by asimpl in H. }
+  { move=>A m1 m1' m2 m2' n n' s pm1 ihm1 pm2 ihm2 pn ihn σ.
+    asimpl.
+    pose proof (pstep_iota1 A.[up σ] s (ihm1 σ) (ihm2 σ) (ihn (upn 2 σ))).
+    by asimpl in H. }
+  { move=>A H H' m m' pH ihH pm ihm σ.
+    asimpl.
+    pose proof (pstep_jelim A.[upn 3 σ] (ihH (up σ)) (ihm σ)).
+    by asimpl in H0. }
 Qed.
 
 Definition psstep (σ τ : var -> term) := forall x, pstep (σ x) (τ x).
 
-Lemma psstep_refl σ : psstep σ σ.
-Proof with eauto using pstep_refl. elim... Qed.
+Lemma psstep_reflexive σ : psstep σ σ.
+Proof with eauto using pstep_reflexive. elim... Qed.
 
 Lemma psstep_up σ τ : psstep σ τ -> psstep (up σ) (up τ).
-Proof with eauto using pstep, pstep_refl.
+Proof with eauto using pstep, pstep_reflexive.
   move=> A [|n] //=. asimpl... asimpl; apply: pstep_subst. exact: A.
 Qed.
 
@@ -262,14 +595,27 @@ Lemma pstep_compat m n σ τ :
   pstep m n -> psstep σ τ -> pstep m.[σ] n.[τ].
 Proof with eauto 6 using pstep, psstep_up.
   move=> ps. elim: ps σ τ=>{m n}...
-  { move=> A m m' n n' s ps1 ih1 ps2 ih2 σ τ pss.
-    asimpl.
+  { move=> A m m' n n' s ps1 ih1 ps2 ih2 σ τ pss. asimpl.
     pose proof (pstep_beta0 A.[σ] s (ih1 _ _ (psstep_up pss)) (ih2 _ _ pss)) as H.
     by asimpl in H. }
-  { move=> A m m' n n' s ps1 ih1 ps2 ih2 σ τ pss.
-    asimpl.
+  { move=> A m m' n n' s ps1 ih1 ps2 ih2 σ τ pss. asimpl.
     pose proof (pstep_beta1 A.[σ] s (ih1 _ _ (psstep_up pss)) (ih2 _ _ pss)) as H.
     by asimpl in H. }
+  { move=>A A' m m' n n' pA ihA pm ihm pn ihn σ τ pss. asimpl.
+    pose proof (pstep_letin (ihA _ _ (psstep_up pss)) (ihm _ _ pss) (ihn _ _ (psstep_upn 2 pss))).
+    by asimpl in H. }
+  { move=>A m1 m1' m2 m2' n n' s pm1 ihm1 pm2 ihm2 pn ihn σ τ pss. asimpl.
+    pose proof (pstep_iota0 A.[up σ] s (ihm1 _ _ pss) (ihm2 _ _ pss) (ihn _ _ (psstep_upn 2 pss))).
+    by asimpl in H. }
+  { move=>A m1 m1' m2 m2' n n' s pm1 ihm1 pm2 ihm2 pn ihn σ τ pss. asimpl.
+    pose proof (pstep_iota1 A.[up σ] s (ihm1 _ _ pss) (ihm2 _ _ pss) (ihn _ _ (psstep_upn 2 pss))).
+    by asimpl in H. }
+  { move=>A A' H H' P P' pA ihA pH ihH pP ihP σ τ pss. asimpl.
+    pose proof (pstep_j (ihA _ _ (psstep_upn 3 pss)) (ihH _ _ (psstep_up pss)) (ihP _ _ pss)).
+    by asimpl in H0. }
+  { move=>A H H' m m' pH ihH pm ihm σ τ pss. asimpl.
+    pose proof (pstep_jelim A.[upn 3 σ] (ihH _ _ (psstep_up pss)) (ihm _ _ pss)).
+    by asimpl in H0. }
 Qed.
 
 Lemma psstep_compat s1 s2 σ τ:
@@ -278,13 +624,13 @@ Proof. move=> A B [|n] //=. Qed.
 
 Lemma pstep_subst_term m n n' :
   pstep n n' -> pstep m.[n/] m.[n'/].
-Proof with eauto using pstep_compat, psstep_refl, psstep_compat.
+Proof with eauto using pstep_compat, psstep_reflexive, psstep_compat.
   move...
 Qed.
 
 Lemma pstep_compat_beta m m' n n' :
   pstep m m' -> pstep n n' -> pstep m.[n/] m'.[n'/].
-Proof with eauto using pstep_compat, psstep_refl, psstep_compat.
+Proof with eauto using pstep_compat, psstep_reflexive, psstep_compat.
   move...
 Qed.
 
@@ -293,7 +639,7 @@ Lemma pstep_diamond m m1 m2 :
 Proof with eauto 6 using
   pstep, pstep_refl,
   pstep_compat, pstep_compat_beta,
-  psstep_compat, psstep_refl.
+  psstep_compat, psstep_reflexive.
   move=>ps. elim: ps m2=>{m m1}...
   { move=>A A' B B' s pA ihA pB ihB m2 p. inv p.
     have[A0 pA1 pA2]:=ihA _ H3.
@@ -341,6 +687,109 @@ Proof with eauto 6 using
     { have[m0 pm1 pm2]:=ihm _ H4.
       have[n0 pn1 pn2]:=ihn _ H5.
       exists (m0.[n0/])... } }
+  { move=>A A' B B' s pA ihA pB ihB m2 p. inv p.
+    have[A0 pA1 pA2]:=ihA _ H3.
+    have[B0 pB1 pB2]:=ihB _ H4.
+    exists (Sig0 A0 B0 s)... }
+  { move=>A A' B B' s pA ihA pB ihB m2 p. inv p.
+    have[A0 pA1 pA2]:=ihA _ H3.
+    have[B0 pB1 pB2]:=ihB _ H4.
+    exists (Sig1 A0 B0 s)... }
+  { move=>m m' n n' s pm ihm pn ihn m2 p. inv p.
+    have[m0 pm1 pm2]:=ihm _ H3.
+    have[n0 pn1 pn2]:=ihn _ H4.
+    exists (Pair0 m0 n0 s)... }
+  { move=>m m' n n' s pm ihm pn ihn m2 p. inv p.
+    have[m0 pm1 pm2]:=ihm _ H3.
+    have[n0 pn1 pn2]:=ihn _ H4.
+    exists (Pair1 m0 n0 s)... }
+  { move=>A A' m m' n n' pA ihA pm ihm pn ihn m2 p. inv p.
+    { have[A0 pA1 pA2]:=ihA _ H2.
+      have[m0 pm1 pm2]:=ihm _ H4.
+      have[n0 pn1 pn2]:=ihn _ H5.
+      exists (LetIn A0 m0 n0)... }
+    { inv pm.
+      have/ihm[mx pm1 pm2]:pstep (Pair0 m1 m0 s) (Pair0 m1' m2' s)...
+      have[n0 pn1 pn2]:=ihn _ H5.
+      inv pm1. inv pm2.
+      exists n0.[n'2,m'/]... }
+    { inv pm.
+      have/ihm[mx pm1 pm2]:pstep (Pair1 m1 m0 s) (Pair1 m1' m2' s)...
+      have[n0 pn1 pn2]:=ihn _ H5.
+      inv pm1. inv pm2.
+      exists n0.[n'2,m'/]... } }
+  { move=>A m1 m1' m2 m2' n n' s pm1 ihm1 pm2 ihm2 pn ihn m0 p. inv p.
+    { inv H4.
+      have[m1x pm11 pm12]:=ihm1 _ H6.
+      have[m2x pm21 pm22]:=ihm2 _ H7.
+      have[n0 pn1 pn2]:=ihn _ H5.
+      exists n0.[m2x,m1x/]... }
+    { have[m1x pm11 pm12]:=ihm1 _ H5.
+      have[m2x pm21 pm22]:=ihm2 _ H6.
+      have[n0 pn1 pn2]:=ihn _ H7.
+      exists n0.[m2x,m1x/]... } }
+  { move=>A m1 m1' m2 m2' n n' s pm1 ihm1 pm2 ihm2 pn ihn m0 p. inv p.
+    { inv H4.
+      have[m1x pm11 pm12]:=ihm1 _ H6.
+      have[m2x pm21 pm22]:=ihm2 _ H7.
+      have[n0 pn1 pn2]:=ihn _ H5.
+      exists n0.[m2x,m1x/]... }
+    { have[m1x pm11 pm12]:=ihm1 _ H5.
+      have[m2x pm21 pm22]:=ihm2 _ H6.
+      have[n0 pn1 pn2]:=ihn _ H7.
+      exists n0.[m2x,m1x/]... } }
+  { move=> A A' B B' s pA ihA pB ihB m2 p. inv p.
+    have[A0 pA1 pA2]:=ihA _ H3.
+    have[B0 pB1 pB2]:=ihB _ H4.
+    exists (With A0 B0 s)... }
+  { move=>m m' n n' s pm ihm pn ihn m2 p. inv p.
+    have[m0 pm1 pm2]:=ihm _ H3.
+    have[n0 pn1 pn2]:=ihn _ H4.
+    exists (APair m0 n0 s)... }
+  { move=>m m' pm ihm m2 p. inv p.
+    { have[m0 pm1 pm2]:=ihm _ H0. exists (Fst m0)... }
+    { inv pm.
+      have/ihm[x p1 p2]:pstep (APair m0 n s) (APair m2 n' s)...
+      inv p1. inv p2.
+      exists m'... } }
+  { move=>m m' pm ihm m2 p. inv p.
+    { have[m0 pm1 pm2]:=ihm _ H0. exists (Snd m0)... }
+    { inv pm.
+      have/ihm[x p1 p2]:pstep (APair m0 n s) (APair m'0 m2 s)...
+      inv p1. inv p2.
+      exists n'0... } }
+  { move=>m m' n s pm ihm m2 p. inv p.
+    { inv H0. have[m0 p1 p2]:=ihm _ H4. exists m0... }
+    { have[m0 p1 p2]:=ihm _ H3. exists m0... } }
+  { move=>m m' n s pm ihm m2 p. inv p.
+    { inv H0. have[m0 p1 p2]:=ihm _ H5. exists m0... }
+    { have[m0 p1 p2]:=ihm _ H3. exists m0... } }
+  { move=>A A' m m' n n' pA ihA pm ihm pn ihn m2 p. inv p.
+    have[A0 pA1 pA2]:=ihA _ H2.
+    have[m0 pm1 pm2]:=ihm _ H4.
+    have[n0 pn1 pn2]:=ihn _ H5.
+    exists (Id A0 m0 n0)... }
+  { move=>m m' pm ihm m2 p. inv p.
+    have[m0 p1 p2]:=ihm _ H0.
+    exists (Refl m0)... }
+  { move=>A A' H H' P P' pA ihA pH ihH pP ihP m2 p. inv p.
+    { have[A0 pA1 pA2]:=ihA _ H4.
+      have[H0 pH1 pH2]:=ihH _ H6.
+      have[P0 pP1 pP2]:=ihP _ H7.
+      exists (J A0 H0 P0)... }
+    { inv pP.
+      have[H0 pH1 pH2]:=ihH _ H5.
+      have/ihP[x p1 p2]:pstep (Refl m) (Refl m')...
+      inv p1. inv p2.
+      exists H0.[m'1/]... } }
+  { move=>A H H' m m' pH ihH pm ihm x p. inv p.
+    { inv H7.
+      have[H0 pH1 pH2]:=ihH _ H6.
+      have[m0 pm1 pm2]:=ihm _ H1.
+      exists H0.[m0/]... }
+    { have[H0 pH1 pH2]:=ihH _ H5.
+      have[m0 pm1 pm2]:=ihm _ H6.
+      exists H0.[m0/]... } }
 Qed.
 
 Lemma strip m m1 m2 :
@@ -379,6 +828,12 @@ Proof.
   apply confluence.
 Qed.
 
+Lemma sta_red_var_inv x y : Var x ~>* y -> y = Var x.
+Proof.
+  elim=>//{} y z r1 e r2; subst.
+  inv r2.
+Qed.
+
 Lemma sta_red_sort_inv s A :
   Sort s ~>* A -> A = Sort s.
 Proof.
@@ -393,7 +848,7 @@ Lemma sta_red_pi0_inv A B s x :
 Proof.
   elim.
   exists A. exists B=>//.
-  move=> y z rd [A'[B'[r1[r2 e]]]] st; subst.
+  move=> y z rd[A'[B'[r1[r2 e]]]] st; subst.
   inv st.
   exists A'0. exists B'.
   repeat constructor; eauto.
@@ -410,7 +865,7 @@ Lemma sta_red_pi1_inv A B s x :
 Proof.
   elim.
   exists A. exists B=>//.
-  move=> y z rd [A'[B'[r1[r2 e]]]] st; subst.
+  move=> y z rd[A'[B'[r1[r2 e]]]] st; subst.
   inv st.
   exists A'0. exists B'.
   repeat constructor; eauto.
@@ -420,12 +875,6 @@ Proof.
   apply: starSE; eauto.
 Qed.
 
-Lemma sta_red_var_inv x y : Var x ~>* y -> y = Var x.
-Proof.
-  elim=>//{} y z r1 e r2; subst.
-  inv r2.
-Qed.
-
 Lemma sta_red_lam0_inv A m x s :
   Lam0 A m s ~>* x ->
   exists A' m',
@@ -433,7 +882,7 @@ Lemma sta_red_lam0_inv A m x s :
 Proof.
   elim.
   exists A. exists m=>//.
-  move=>y z r1 [A'[m'[rA[rm e]]]] r2. subst.
+  move=>y z r1[A'[m'[rA[rm e]]]] r2. subst.
   inv r2.
   exists A'0. exists m'. eauto using star.
   exists A'. exists m'0. eauto using star.
@@ -446,10 +895,144 @@ Lemma sta_red_lam1_inv A m x s :
 Proof.
   elim.
   exists A. exists m=>//.
-  move=>y z r1 [A'[m'[rA[rm e]]]] r2. subst.
+  move=>y z r1[A'[m'[rA[rm e]]]] r2. subst.
   inv r2.
   exists A'0. exists m'. eauto using star.
   exists A'. exists m'0. eauto using star.
+Qed.
+
+Lemma sta_red_sig0_inv A B s x :
+  Sig0 A B s ~>* x ->
+  exists A' B',
+    A ~>* A' /\ B ~>* B' /\ x = Sig0 A' B' s.
+Proof.
+  elim.
+  exists A. exists B=>//.
+  move=> y z rd[A'[B'[r1[r2 e]]]] st; subst.
+  inv st.
+  exists A'0. exists B'.
+  repeat constructor; eauto.
+  apply: starSE; eauto.
+  exists A'. exists B'0.
+  repeat constructor; eauto.
+  apply: starSE; eauto.
+Qed.
+
+Lemma sta_red_sig1_inv A B s x :
+  Sig1 A B s ~>* x ->
+  exists A' B',
+    A ~>* A' /\ B ~>* B' /\ x = Sig1 A' B' s.
+Proof.
+  elim.
+  exists A. exists B=>//.
+  move=> y z rd[A'[B'[r1[r2 e]]]] st; subst.
+  inv st.
+  exists A'0. exists B'.
+  repeat constructor; eauto.
+  apply: starSE; eauto.
+  exists A'. exists B'0.
+  repeat constructor; eauto.
+  apply: starSE; eauto.
+Qed.
+
+Lemma sta_red_pair0_inv m n s x :
+  Pair0 m n s ~>* x ->
+  exists m' n',
+    m ~>* m' /\ n ~>* n' /\ x = Pair0 m' n' s.
+Proof.
+  elim.
+  exists m. exists n=>//.
+  move=> y z rd[m'[n'[r1[r2 e]]]] st; subst.
+  inv st.
+  exists m'0. exists n'.
+  repeat constructor; eauto.
+  apply: starSE; eauto.
+  exists m'. exists n'0.
+  repeat constructor; eauto.
+  apply: starSE; eauto.
+Qed.
+
+Lemma sta_red_pair1_inv m n s x :
+  Pair1 m n s ~>* x ->
+  exists m' n',
+    m ~>* m' /\ n ~>* n' /\ x = Pair1 m' n' s.
+Proof.
+  elim.
+  exists m. exists n=>//.
+  move=> y z rd[m'[n'[r1[r2 e]]]] st; subst.
+  inv st.
+  exists m'0. exists n'.
+  repeat constructor; eauto.
+  apply: starSE; eauto.
+  exists m'. exists n'0.
+  repeat constructor; eauto.
+  apply: starSE; eauto.
+Qed.
+
+Lemma sta_red_with_inv A B s x :
+  With A B s ~>* x ->
+  exists A' B',
+    A ~>* A' /\ B ~>* B' /\ x = With A' B' s.
+Proof.
+  elim.
+  exists A. exists B=>//.
+  move=> y z rd[A'[B'[r1[r2 e]]]] st; subst.
+  inv st.
+  exists A'0. exists B'.
+  repeat constructor; eauto.
+  apply: starSE; eauto.
+  exists A'. exists B'0.
+  repeat constructor; eauto.
+  apply: starSE; eauto.
+Qed.
+
+Lemma sta_red_apair_inv m n s x :
+  APair m n s ~>* x ->
+  exists m' n',
+    m ~>* m' /\ n ~>* n' /\ x = APair m' n' s.
+Proof.
+  elim.
+  exists m. exists n=>//.
+  move=> y z rd[m'[n'[r1[r2 e]]]] st; subst.
+  inv st.
+  exists m'0. exists n'.
+  repeat constructor; eauto.
+  apply: starSE; eauto.
+  exists m'. exists n'0.
+  repeat constructor; eauto.
+  apply: starSE; eauto.
+Qed.
+
+Lemma sta_red_id_inv A m n x :
+  Id A m n ~>* x ->
+  exists A' m' n',
+    A ~>* A' /\ m ~>* m' /\ n ~>* n' /\ x = Id A' m' n'.
+Proof.
+  elim.
+  exists A. exists m. exists n=>//.
+  move=>y z rd[A'[m'[n'[r1[r2[r3 e]]]]]] st; subst.
+  inv st.
+  exists A'0. exists m'. exists n'.
+  repeat constructor; eauto.
+  apply: starSE; eauto.
+  exists A'. exists m'0. exists n'.
+  repeat constructor; eauto.
+  apply: starSE; eauto.
+  exists A'. exists m'. exists n'0.
+  repeat constructor; eauto.
+  apply: starSE; eauto.
+Qed.
+
+Lemma sta_red_refl_inv m x :
+  Refl m ~>* x ->
+  exists m', m ~>* m' /\ x = Refl m'.
+Proof.
+  elim.
+  exists m=>//.
+  move=>y z rd[m'[r e]] st; subst.
+  inv st. exists m'0.
+  repeat constructor; eauto.
+  apply: starSE; eauto.
 Qed.
 
 Lemma sort_inj s1 s2 :
@@ -490,14 +1073,89 @@ Proof.
   apply: conv_sym. by apply: star_conv.
 Qed.
 
+Lemma sig0_inj A A' B B' s s' :
+  Sig0 A B s === Sig0 A' B' s' ->
+    A === A' /\ B === B' /\ s = s'.
+Proof.
+  move/church_rosser=>
+    [x/sta_red_sig0_inv[A1[B1[rA1[rB1->]]]]
+      /sta_red_sig0_inv[A2[B2[rA2[rB2[]]]]]] eA eB es; subst.
+  repeat split.
+  apply: conv_trans.
+  apply: star_conv. by apply: rA1.
+  apply: conv_sym. by apply: star_conv.
+  apply: conv_trans.
+  apply: star_conv. by apply: rB1.
+  apply: conv_sym. by apply: star_conv.
+Qed.
+
+Lemma sig1_inj A A' B B' s s' :
+  Sig1 A B s === Sig1 A' B' s' ->
+    A === A' /\ B === B' /\ s = s'.
+Proof.
+  move/church_rosser=>
+    [x/sta_red_sig1_inv[A1[B1[rA1[rB1->]]]]
+      /sta_red_sig1_inv[A2[B2[rA2[rB2[]]]]]] eA eB es; subst.
+  repeat split.
+  apply: conv_trans.
+  apply: star_conv. by apply: rA1.
+  apply: conv_sym. by apply: star_conv.
+  apply: conv_trans.
+  apply: star_conv. by apply: rB1.
+  apply: conv_sym. by apply: star_conv.
+Qed.
+
+Lemma with_inj A A' B B' s s' :
+  With A B s === With A' B' s' ->
+    A === A' /\ B === B' /\ s = s'.
+Proof.
+  move/church_rosser=>
+    [x/sta_red_with_inv[A1[B1[rA1[rB1->]]]]
+      /sta_red_with_inv[A2[B2[rA2[rB2[]]]]]] eA eB es; subst.
+  repeat split.
+  apply: conv_trans.
+  apply: star_conv. by apply: rA1.
+  apply: conv_sym. by apply: star_conv.
+  apply: conv_trans.
+  apply: star_conv. by apply: rB1.
+  apply: conv_sym. by apply: star_conv.
+Qed.
+
+Lemma id_inj A A' m m' n n' :
+  Id A m n === Id A' m' n' ->
+    A === A' /\ m === m' /\ n === n'.
+Proof.
+  move/church_rosser=>
+    [x/sta_red_id_inv[A1[m1[n1[rA1[rm1[rn1->]]]]]]
+      /sta_red_id_inv[A2[m2[n2[rA2[rm2[rn2[]]]]]]]] eA em en; subst.
+  repeat split.
+  apply: conv_trans.
+  apply: star_conv. by apply: rA1.
+  apply: conv_sym. by apply: star_conv.
+  apply: conv_trans.
+  apply: star_conv. by apply: rm1.
+  apply: conv_sym. by apply: star_conv.
+  apply: conv_trans.
+  apply: star_conv. by apply: rn1.
+  apply: conv_sym. by apply: star_conv.
+Qed.
+
 Ltac red_inv m H :=
   match m with
-  | Var  => apply sta_red_var_inv in H
-  | Sort => apply sta_red_sort_inv in H
-  | Pi0  => apply sta_red_pi0_inv in H
-  | Pi1  => apply sta_red_pi1_inv in H
-  | Lam0 => apply sta_red_lam0_inv in H
-  | Lam1 => apply sta_red_lam1_inv in H
+  | Var   => apply sta_red_var_inv in H
+  | Sort  => apply sta_red_sort_inv in H
+  | Pi0   => apply sta_red_pi0_inv in H
+  | Pi1   => apply sta_red_pi1_inv in H
+  | Lam0  => apply sta_red_lam0_inv in H
+  | Lam1  => apply sta_red_lam1_inv in H
+  | Sig0  => apply sta_red_sig0_inv in H
+  | Sig1  => apply sta_red_sig1_inv in H
+  | Pair0 => apply sta_red_pair0_inv in H
+  | Pair1 => apply sta_red_pair1_inv in H
+  | With  => apply sta_red_with_inv in H
+  | APair => apply sta_red_apair_inv in H
+  | Id    => apply sta_red_id_inv in H
+  | Refl  => apply sta_red_refl_inv in H
   end.
 
 Ltac solve_conv' :=
