coq/sta_step.v
@@ -8,40 +8,122 @@ Unset Printing Implicit Defensive.
 
 Reserved Notation "m ~> n" (at level 30).
 Inductive sta_step : term -> term -> Prop :=
-| sta_pi0L A A' B s :
+| sta_step_pi0L A A' B s :
   A ~> A' ->
   Pi0 A B s ~> Pi0 A' B s
-| sta_pi1L A A' B s :
+| sta_step_pi1L A A' B s :
   A ~> A' ->
   Pi1 A B s ~> Pi1 A' B s
-| sta_pi0R A B B' s :
+| sta_step_pi0R A B B' s :
   B ~> B' ->
   Pi0 A B s ~> Pi0 A B' s
-| sta_pi1R A B B' s :
+| sta_step_pi1R A B B' s :
   B ~> B' ->
   Pi1 A B s ~> Pi1 A B' s
-| sta_lam0L A A' m s :
+| sta_step_lam0L A A' m s :
   A ~> A' ->
   Lam0 A m s ~> Lam0 A' m s
-| sta_lam1L A A' m s :
+| sta_step_lam1L A A' m s :
   A ~> A' ->
   Lam1 A m s ~> Lam1 A' m s
-| sta_lam0R A m m' s :
+| sta_step_lam0R A m m' s :
   m ~> m' ->
   Lam0 A m s ~> Lam0 A m' s
-| sta_lam1R A m m' s :
+| sta_step_lam1R A m m' s :
   m ~> m' ->
   Lam1 A m s ~> Lam1 A m' s
-| sta_appL m m' n :
+| sta_step_appL m m' n :
   m ~> m' ->
   App m n ~> App m' n
-| sta_appR m n n' :
+| sta_step_appR m n n' :
   n ~> n' ->
   App m n ~> App m n'
-| sta_beta0 A m n s :
+| sta_step_beta0 A m n s :
   App (Lam0 A m s) n ~> m.[n/]
-| sta_beta1 A m n s :
+| sta_step_beta1 A m n s :
   App (Lam1 A m s) n ~> m.[n/]
+| sta_step_sig0L A A' B s :
+  A ~> A' ->
+  Sig0 A B s ~> Sig0 A' B s
+| sta_step_sig0R A B B' s :
+  B ~> B' ->
+  Sig0 A B s ~> Sig0 A B' s
+| sta_step_sig1L A A' B s :
+  A ~> A' ->
+  Sig1 A B s ~> Sig1 A' B s
+| sta_step_sig1R A B B' s :
+  B ~> B' ->
+  Sig1 A B s ~> Sig1 A B' s
+| sta_step_pair0L m m' n s :
+  m ~> m' ->
+  Pair0 m n s ~> Pair0 m' n s
+| sta_step_pair0R m n n' s :
+  n ~> n' ->
+  Pair0 m n s ~> Pair0 m n' s
+| sta_step_pair1L m m' n s :
+  m ~> m' ->
+  Pair1 m n s ~> Pair1 m' n s
+| sta_step_pair1R m n n' s :
+  n ~> n' ->
+  Pair1 m n s ~> Pair1 m n' s
+| sta_step_letinA A A' m n :
+  A ~> A' ->
+  LetIn A m n ~> LetIn A' m n
+| sta_step_letinL A m m' n :
+  m ~> m' ->
+  LetIn A m n ~> LetIn A m' n
+| sta_step_letinR A m n n' :
+  n ~> n' ->
+  LetIn A m n ~> LetIn A m n'
+| sta_step_iota0 A m1 m2 n s :
+  LetIn A (Pair0 m1 m2 s) n ~> n.[m2,m1/]
+| sta_step_iota1 A m1 m2 n s :
+  LetIn A (Pair1 m1 m2 s) n ~> n.[m2,m1/]
+| sta_step_withL A A' B s :
+  A ~> A' ->
+  With A B s ~> With A' B s
+| sta_step_withR A B B' s :
+  B ~> B' ->
+  With A B s ~> With A B' s
+| sta_step_apairL m m' n s :
+  m ~> m' ->
+  APair m n s ~> APair m' n s
+| sta_step_apairR m n n' s :
+  n ~> n' ->
+  APair m n s ~> APair m n' s
+| sta_step_fst m m' :
+  m ~> m' ->
+  Fst m ~> Fst m'
+| sta_step_snd m m' :
+  m ~> m' ->
+  Snd m ~> Snd m'
+| sta_step_proj1 m n s :
+  Fst (APair m n s) ~> m
+| sta_step_proj2 m n s :
+  Snd (APair m n s) ~> n
+| sta_step_idA A A' m n :
+  A ~> A' ->
+  Id A m n ~> Id A' m n
+| sta_step_idL A m m' n :
+  m ~> m' ->
+  Id A m n ~> Id A m' n
+| sta_step_idR A m n n' :
+  n ~> n' ->
+  Id A m n ~> Id A m n'
+| sta_step_refl m m' :
+  m ~> m' ->
+  Refl m ~> Refl m'
+| sta_step_jA A A' H P :
+  A ~> A' ->
+  J A H P ~> J A' H P
+| sta_step_jH A H H' P :
+  H ~> H' ->
+  J A H P ~> J A H' P
+| sta_step_jP A H P P' :
+  P ~> P' ->
+  J A H P ~> J A H P'
+| sta_step_jelim A H m :
+  J A H (Refl m) ~> H.[m/]
 where "m ~> n" := (sta_step m n).
 
 Notation sta_red := (star sta_step).
