old/coq1/sta_type.v
@@ -38,64 +38,6 @@ Inductive sta0_type : sta_ctx -> term -> term -> Prop :=
   sta0_type Γ m (Pi1 A B s) ->
   sta0_type Γ n A ->
   sta0_type Γ (App m n) B.[n/]
-| sta0_sig0 Γ A B s r t :
-  s ⊑ t ->
-  sta0_type Γ A (Sort s) ->
-  sta0_type (A :: Γ) B (Sort r) ->
-  sta0_type Γ (Sig0 A B t) (Sort t)
-| sta0_sig1 Γ A B s r t :
-  s ⊑ t ->
-  r ⊑ t ->
-  sta0_type Γ A (Sort s) ->
-  sta0_type (A :: Γ) B (Sort r) ->
-  sta0_type Γ (Sig1 A B t) (Sort t)
-| sta0_pair0 Γ A B m n t :
-  sta0_type Γ (Sig0 A B t) (Sort t) ->
-  sta0_type Γ m A ->
-  sta0_type Γ n B.[m/] ->
-  sta0_type Γ (Pair0 m n t) (Sig0 A B t)
-| sta0_pair1 Γ A B m n t :
-  sta0_type Γ (Sig1 A B t) (Sort t) ->
-  sta0_type Γ m A ->
-  sta0_type Γ n B.[m/] ->
-  sta0_type Γ (Pair1 m n t) (Sig1 A B t)
-| sta0_letin0 Γ A B C m n s t :
-  sta0_type (Sig0 A B t :: Γ) C (Sort s) ->
-  sta0_type Γ m (Sig0 A B t) ->
-  sta0_type (B :: A :: Γ) n C.[Pair0 (Var 1) (Var 0) t .: ren (+2)] ->
-  sta0_type Γ (LetIn C m n) C.[m/]
-| sta0_letin1 Γ A B C m n s t :
-  sta0_type (Sig1 A B t :: Γ) C (Sort s) ->
-  sta0_type Γ m (Sig1 A B t) ->
-  sta0_type (B :: A :: Γ) n C.[Pair1 (Var 1) (Var 0) t .: ren (+2)] ->
-  sta0_type Γ (LetIn C m n) C.[m/]
-| sta0_with Γ A B s r t :
-  sta0_type Γ A (Sort s) ->
-  sta0_type Γ B (Sort r) ->
-  sta0_type Γ (With A B t) (Sort t)
-| sta0_apair Γ A B m n t :
-  sta0_type Γ m A ->
-  sta0_type Γ n B ->
-  sta0_type Γ (APair m n t) (With A B t)
-| sta0_fst Γ A B m t :
-  sta0_type Γ m (With A B t) ->
-  sta0_type Γ (Fst m) A
-| sta0_snd Γ A B m t :
-  sta0_type Γ m (With A B t) ->
-  sta0_type Γ (Snd m) B
-| sta0_id Γ A m n s :
-  sta0_type Γ A (Sort s) ->
-  sta0_type Γ m A ->
-  sta0_type Γ n A ->
-  sta0_type Γ (Id A m n) (Sort U)
-| sta0_refl Γ A m :
-  sta0_type Γ m A ->
-  sta0_type Γ (Refl m) (Id A m m)
-| sta0_j Γ A B H P m n s :
-  sta0_type (Id A.[ren (+2)] (Var 1) (Var 0) :: A.[ren (+1)] :: A :: Γ) B (Sort s) ->
-  sta0_type (A :: Γ) H B.[Refl (Var 0) .: Var 0 .: Var 0 .: ren (+1)] ->
-  sta0_type Γ P (Id A m n) ->
-  sta0_type Γ (J B H P) B.[P,n,m/]
 | sta0_conv Γ A B m s :
   A === B ->
   sta0_type Γ m A ->
@@ -147,64 +89,6 @@ Inductive sta_type : sta_ctx -> term -> term -> Prop :=
   Γ ⊢ m : Pi1 A B s ->
   Γ ⊢ n : A ->
   Γ ⊢ App m n : B.[n/]
-| sta_sig0 Γ A B s r t :
-  s ⊑ t ->
-  Γ ⊢ A : Sort s ->
-  (A :: Γ) ⊢ B : Sort r ->
-  Γ ⊢ Sig0 A B t : Sort t
-| sta_sig1 Γ A B s r t :
-  s ⊑ t ->
-  r ⊑ t ->
-  Γ ⊢ A : Sort s ->
-  (A :: Γ) ⊢ B : Sort r ->
-  Γ ⊢ Sig1 A B t : Sort t
-| sta_pair0 Γ A B m n t :
-  Γ ⊢ Sig0 A B t : Sort t ->
-  Γ ⊢ m : A ->
-  Γ ⊢ n : B.[m/] ->
-  Γ ⊢ Pair0 m n t : Sig0 A B t
-| sta_pair1 Γ A B m n t :
-  Γ ⊢ Sig1 A B t : Sort t ->
-  Γ ⊢ m : A ->
-  Γ ⊢ n : B.[m/] ->
-  Γ ⊢ Pair1 m n t : Sig1 A B t
-| sta_letin0 Γ A B C m n s t :
-  (Sig0 A B t :: Γ) ⊢ C : Sort s ->
-  Γ ⊢ m : Sig0 A B t ->
-  (B :: A :: Γ) ⊢ n : C.[Pair0 (Var 1) (Var 0) t .: ren (+2)] ->
-  Γ ⊢ LetIn C m n : C.[m/]
-| sta_letin1 Γ A B C m n s t :
-  (Sig1 A B t :: Γ) ⊢ C : Sort s ->
-  Γ ⊢ m : Sig1 A B t ->
-  (B :: A :: Γ) ⊢ n : C.[Pair1 (Var 1) (Var 0) t .: ren (+2)] ->
-  Γ ⊢ LetIn C m n : C.[m/]
-| sta_with Γ A B s r t :
-  Γ ⊢ A : Sort s ->
-  Γ ⊢ B : Sort r ->
-  Γ ⊢ With A B t : Sort t
-| sta_apair Γ A B m n t :
-  Γ ⊢ m : A ->
-  Γ ⊢ n : B ->
-  Γ ⊢ APair m n t : With A B t
-| sta_fst Γ A B m t :
-  Γ ⊢ m : With A B t ->
-  Γ ⊢ Fst m : A
-| sta_snd Γ A B m t :
-  Γ ⊢ m : With A B t ->
-  Γ ⊢ Snd m : B
-| sta_id Γ A m n s :
-  Γ ⊢ A : Sort s ->
-  Γ ⊢ m : A ->
-  Γ ⊢ n : A ->
-  Γ ⊢ Id A m n : Sort U
-| sta_refl Γ A m :
-  Γ ⊢ m : A ->
-  Γ ⊢ Refl m : Id A m m
-| sta_j Γ A B H P m n s :
-  (Id A.[ren (+2)] (Var 1) (Var 0) :: A.[ren (+1)] :: A :: Γ) ⊢ B : Sort s ->
-  (A :: Γ) ⊢ H : B.[Refl (Var 0) .: Var 0 .: Var 0 .: ren (+1)] ->
-  Γ ⊢ P : Id A m n ->
-  Γ ⊢ J B H P : B.[P,n,m/]
 | sta_conv Γ A B m s :
   A === B ->
   Γ ⊢ m : A ->
@@ -241,7 +125,6 @@ Proof with eauto using sta0_type, sta0_wf.
     apply: sta0_lam1... }
   Unshelve. eauto.
 Qed.
-Hint Resolve sta_sta0_type.
 
 Lemma sta0_sta_type Γ m A : sta0_type Γ m A -> Γ ⊢ m : A.
 Proof with eauto using sta_type, sta_wf.
