coq/dyn_prog.v
@@ -17,12 +17,20 @@ Proof with eauto.
   { move=>Γ Δ A B m s k tym ihm A0 B0 s0
       e1 e2/pi0_inj[eq1[eq2 e3]] vl; subst.
     exists A. exists m... }
-  { move=>Γ Δ A B m s t k tym _ A0 B0 s0 e1 e2 eq.
-    exfalso. solve_conv. }
+  { move=>*. exfalso. solve_conv. }
   { move=>Γ Δ A B m n s tym ihm tyn A0 B0
       s0 e1 e2 eq vl. inv vl. }
   { move=>Γ Δ1 Δ2 Δ A B m n s mrg tym _ tyn _ A0 B0
       s0 e1 e2 eq vl. inv vl. }
+  { move=>*. exfalso. solve_conv. }
+  { move=>*. exfalso. solve_conv. }
+  { move=>Γ Δ1 Δ2 Δ A B C m n s r t mrg tyC tym ihm tyn ihn A0 B0
+      s0 e1 e2 eq vl. inv vl. }
+  { move=>Γ Δ1 Δ2 Δ A B C m n s r1 r2 t mrg tyC tym ihm tyn ihn A0 B0
+      s0 e1 e2 eq vl. inv vl. }
+  { move=>*. exfalso. solve_conv. }
+  { move=>Γ Δ A B m t tym ihm A0 B0 s e1 e2 eq vl. inv vl. }
+  { move=>Γ Δ A B m t tym ihm A0 B0 s e1 e2 eq vl. inv vl. }
   { move=>Γ Δ A B m s eq1 tym ihm tyB A0 B0 s0 e1 e2 eq2 vl.
     apply: ihm...
     apply: conv_trans... }
@@ -45,6 +53,99 @@ Proof with eauto.
       s0 e1 e2 eq vl. inv vl. }
   { move=>Γ Δ1 Δ2 Δ A B m n s mrg tym _ tyn _ A0 B0
       s0 e1 e2 eq vl. inv vl. }
+  { move=>*. exfalso. solve_conv. }
+  { move=>*. exfalso. solve_conv. }
+  { move=>Γ Δ1 Δ2 Δ A B C m n s r t mrg tyC tym ihm tyn ihn A0 B0
+      s0 e1 e2 eq vl. inv vl. }
+  { move=>Γ Δ1 Δ2 Δ A B C m n s r1 r2 t mrg tyC tym ihm tyn ihn A0 B0
+      s0 e1 e2 eq vl. inv vl. }
+  { move=>*. exfalso. solve_conv. }
+  { move=>Γ Δ A B m t tym ihm A0 B0 s e1 e2 eq vl. inv vl. }
+  { move=>Γ Δ A B m t tym ihm A0 B0 s e1 e2 eq vl. inv vl. }
+  { move=>Γ Δ A B m s eq1 tym ihm tyB A0 B0 s0 e1 e2 eq2 vl.
+    apply: ihm...
+    apply: conv_trans... }
+Qed.
+
+Lemma dyn_sig0_canonical m A B C s :
+  nil ; nil ⊢ m : C -> C === Sig0 A B s -> dyn_val m ->
+  exists m1 m2, m = Pair0 m1 m2 s.
+Proof with eauto.
+  move e1:(nil)=>Γ.
+  move e2:(nil)=>Δ ty.
+  elim: ty A B s e1 e2=>//{Γ Δ m C}.
+  { move=>Γ Δ x s A wf shs dhs A0 B s0 e1 e2; subst. inv shs. }
+  { move=>*. exfalso. solve_conv. }
+  { move=>*. exfalso. solve_conv. }
+  { move=>Γ Δ A B m n s tym ihm tyn A0 B0 s0 e1 e2 eq vl. inv vl. }
+  { move=>Γ Δ1 Δ2 Δ A B m n s mrg tym ihm tyn ihn A0 B0 s0 e1 e2 eq vl. inv vl. }
+  { move=>Γ Δ A B m n t tyS tym ihm tyn A0 B0 s
+      e1 e2/sig0_inj[eq1[eq2 e3]] vl; subst.
+    exists m. exists n... }
+  { move=>*. exfalso. solve_conv. }
+  { move=>Γ Δ1 Δ2 Δ A B C m n s r t mrg tyC tym ihm tyn ihn A0 B0
+      s0 e1 e2 eq vl. inv vl. }
+  { move=>Γ Δ1 Δ2 Δ A B C m n s r1 r2 t mrg tyC tym ihm tyn ihn A0 B0
+      s0 e1 e2 eq vl. inv vl. }
+  { move=>*. exfalso. solve_conv. }
+  { move=>Γ Δ A B m t tym ihm A0 B0 s e1 e2 eq vl. inv vl. }
+  { move=>Γ Δ A B m t tym ihm A0 B0 s e1 e2 eq vl. inv vl. }
+  { move=>Γ Δ A B m s eq1 tym ihm tyB A0 B0 s0 e1 e2 eq2 vl.
+    apply: ihm...
+    apply: conv_trans... }
+Qed.
+
+Lemma dyn_sig1_canonical m A B C s :
+  nil ; nil ⊢ m : C -> C === Sig1 A B s -> dyn_val m ->
+  exists m1 m2, m = Pair1 m1 m2 s.
+Proof with eauto.
+  move e1:(nil)=>Γ.
+  move e2:(nil)=>Δ ty.
+  elim: ty A B s e1 e2=>//{Γ Δ m C}.
+  { move=>Γ Δ x s A wf shs dhs A0 B s0 e1 e2; subst. inv shs. }
+  { move=>*. exfalso. solve_conv. }
+  { move=>*. exfalso. solve_conv. }
+  { move=>Γ Δ A B m n s tym ihm tyn A0 B0 s0 e1 e2 eq vl. inv vl. }
+  { move=>Γ Δ1 Δ2 Δ A B m n s mrg tym ihm tyn ihn A0 B0 s0 e1 e2 eq vl. inv vl. }
+  { move=>*. exfalso. solve_conv. }
+  { move=>Γ Δ1 Δ2 Δ A B m n t mrg tyS tym ihm tyn ihn A0 B0 s
+      e1 e2/sig1_inj[eq1[eq2 e3]]vl; subst.
+    exists m. exists n... }
+  { move=>Γ Δ1 Δ2 Δ A B C m n s r t mrg tyC tym ihm tyn ihn A0 B0
+      s0 e1 e2 eq vl. inv vl. }
+  { move=>Γ Δ1 Δ2 Δ A B C m n s r1 r2 t mrg tyC tym ihm tyn ihn A0 B0
+      s0 e1 e2 eq vl. inv vl. }
+  { move=>*. exfalso. solve_conv. }
+  { move=>Γ Δ A B m t tym ihm A0 B0 s e1 e2 eq vl. inv vl. }
+  { move=>Γ Δ A B m t tym ihm A0 B0 s e1 e2 eq vl. inv vl. }
+  { move=>Γ Δ A B m s eq1 tym ihm tyB A0 B0 s0 e1 e2 eq2 vl.
+    apply: ihm...
+    apply: conv_trans... }
+Qed.
+
+Lemma dyn_with_canonical m A B C s :
+  nil ; nil ⊢ m : C -> C === With A B s -> dyn_val m ->
+  exists m1 m2, m = APair m1 m2 s.
+Proof with eauto.
+  move e1:(nil)=>Γ.
+  move e2:(nil)=>Δ ty.
+  elim: ty A B s e1 e2=>//{Γ Δ m C}.
+  { move=>Γ Δ x s A wf shs dhs A0 B s0 e1 e2; subst. inv shs. }
+  { move=>*. exfalso. solve_conv. }
+  { move=>*. exfalso. solve_conv. }
+  { move=>Γ Δ A B m n s tym ihm tyn A0 B0 s0 e1 e2 eq vl. inv vl. }
+  { move=>Γ Δ1 Δ2 Δ A B m n s mrg tym ihm tyn ihn A0 B0 s0 e1 e2 eq vl. inv vl. }
+  { move=>*. exfalso. solve_conv. }
+  { move=>*. exfalso. solve_conv. }
+  { move=>Γ Δ1 Δ2 Δ A B C m n s r t mrg tyC tym ihm tyn ihn A0 B0
+      s0 e1 e2 eq vl. inv vl. }
+  { move=>Γ Δ1 Δ2 Δ A B C m n s r1 r2 t mrg tyC tym ihm tyn ihn A0 B0
+      s0 e1 e2 eq vl. inv vl. }
+  { move=>Γ Δ A B m n t k tym ihm tyn ihn A0 B0 s
+      e1 e2/with_inj[eq1[eq2 e3]]vl; subst.
+    exists m. exists n... }
+  { move=>Γ Δ A B m t tym ihm A0 B0 s e1 e2 eq vl. inv vl. }
+  { move=>Γ Δ A B m t tym ihm A0 B0 s e1 e2 eq vl. inv vl. }
   { move=>Γ Δ A B m s eq1 tym ihm tyB A0 B0 s0 e1 e2 eq2 vl.
     apply: ihm...
     apply: conv_trans... }
@@ -72,5 +173,37 @@ Proof with eauto using dyn_step, dyn_val.
       exists (App m n')...
       have[A0[n0 e]]:=dyn_pi1_canonical tym (convR _ _) vlm.
       subst. exists (n0.[n/])... } }
+  { move=>Γ Δ A B m n t tyS tym ihm tyn e1 e2; subst.
+    have[[m' stm]|vlm]:=ihm erefl erefl.
+    { left. exists (Pair0 m' n t)... }
+    { right... } }
+  { move=>Γ Δ1 Δ2 Δ A B m n t mrg tyS tym ihm tyn ihn e1 e2; subst.
+    inv mrg.
+    have[[m' stm]|vlm]:=ihm erefl erefl.
+    { left. exists (Pair1 m' n t)... }
+    { have[[n' stn]|vln]:=ihn erefl erefl.
+      { left. exists (Pair1 m n' t)... }
+      { right... } } }
+  { move=>Γ Δ1 Δ2 Δ A B C m n s r t mrg tyC tym ihm tyn ihn e1 e2; subst.
+    inv mrg. have[[m' stm]|vlm]:=ihm erefl erefl.
+    { left. exists (LetIn C m' n)... }
+    { have[m1[m2 e]]:=dyn_sig0_canonical tym (convR _ _) vlm. subst.
+      left. exists n.[m2,m1/]... } }
+  { move=>Γ Δ1 Δ2 Δ A B C m n s r1 r2 t mrg tyC tym ihm tyn ihn e1 e2; subst.
+    inv mrg. have[[m' stm]|vlm]:=ihm erefl erefl.
+    { left. exists (LetIn C m' n)... }
+    { have[m1[m2 e]]:=dyn_sig1_canonical tym (convR _ _) vlm. subst.
+      left. exists n.[m2,m1/]... } }
+  { move=>Γ Δ A B m n t k tym ihm tyn ihn e1 e2; subst. right... }
+  { move=>Γ Δ A B m t tym ihm e1 e2; subst.
+    have[[m' stm]|vlm]:=ihm erefl erefl.
+    { left. exists (Fst m')... }
+    { have[m1[m2 e]]:=dyn_with_canonical tym (convR _ _) vlm. subst.
+      left. exists m1... } }
+  { move=>Γ Δ A B m t tym ihm e1 e2; subst.
+    have[[m' stm]|vlm]:=ihm erefl erefl.
+    { left. exists (Snd m')... }
+    { have[m1[m2 e]]:=dyn_with_canonical tym (convR _ _) vlm. subst.
+      left. exists m2... } }
   { move=>Γ Δ A B m s eq tym ihm tyB e1 e2; subst... }
 Qed.
