coq/era_prog.v
@@ -22,6 +22,30 @@ Proof with eauto.
   exists m'...
 Qed.
 
+Lemma era_pair0_canonical Γ Δ A m1 m2 n s :
+  Γ ; Δ ⊢ Pair0 m1 m2 s ~ n : A -> exists m1', n = Pair0 m1' Box s.
+Proof with eauto.
+  move e:(Pair0 m1 m2 s)=>x ty. elim: ty m1 m2 s e=>//{Γ Δ x n A}.
+  move=>Γ Δ A B m m' n t tyS erm ihm tyn m1 m2 s[e1 e2 e3]; subst.
+  exists m'...
+Qed.
+
+Lemma era_pair1_canonical Γ Δ A m1 m2 n s :
+  Γ ; Δ ⊢ Pair1 m1 m2 s ~ n : A -> exists m1' m2', n = Pair1 m1' m2' s.
+Proof with eauto.
+  move e:(Pair1 m1 m2 s)=>x ty. elim: ty m1 m2 s e=>//{Γ Δ x n A}.
+  move=>Γ Δ1 Δ2 Δ A B m m' n n' t mrg tyS erm ihm tyn ihn m1 m2 s[e1 e2 e3]; subst.
+  exists m'. exists n'...
+Qed.
+
+Lemma era_apair_canonical Γ Δ A m1 m2 n s :
+  Γ ; Δ ⊢ APair m1 m2 s ~ n : A -> exists m1' m2', n = APair m1' m2' s.
+Proof with eauto.
+  move e:(APair m1 m2 s)=>x ty. elim: ty m1 m2 s e=>//{Γ Δ x n A}.
+  move=>Γ Δ A B m m' n n' t tyS erm ihm tyn ihn m1 m2 s[e1 e2 e3]; subst.
+  exists m'. exists n'...
+Qed.
+
 Lemma era_prog m m' A :
   nil ; nil ⊢ m ~ m' : A -> (exists n', m' ~>> n') \/ dyn_val m'.
 Proof with eauto using dyn_step, dyn_val.
@@ -36,7 +60,7 @@ Proof with eauto using dyn_step, dyn_val.
     have[[x st]|vl]:=ihm erefl erefl.
     { left. exists (App x Box)... }
     { left.
-      have{}vl:=era_dyn_val vl erm.
+      have{}vl:=era_dyn_val erm vl.
       have tym:=era_dyn_type erm.
       have[A0[n0 e]]:=dyn_pi0_canonical tym (convR _ _) vl. subst.
       have[m0 e]:=era_lam0_canonical erm. subst.
@@ -46,10 +70,61 @@ Proof with eauto using dyn_step, dyn_val.
     { left. exists (App mx n')... }
     { left. have[[nx st2]|vln]:=ihn erefl erefl.
       exists (App m' nx)...
-      have{}vlm:=era_dyn_val vlm erm.
+      have{}vlm:=era_dyn_val erm vlm.
       have tym:=era_dyn_type erm.
       have[A0[n0 e]]:=dyn_pi1_canonical tym (convR _ _) vlm. subst.
       have[m0 e]:=era_lam1_canonical erm. subst.
       exists (m0.[n'/])... } }
+  { move=>Γ Δ A B m m' n t tyS erm ihm tyn e1 e2; subst.
+    have[[mx stm]|vlm]:=ihm erefl erefl.
+    { left. exists (Pair0 mx Box t)... }
+    { right... } }
+  { move=>Γ Δ1 Δ2 Δ A B m m' n n' t mrg tyS erm ihm ern ihn e1 e2; subst.
+    inv mrg. have[[mx stm]|vlm]:=ihm erefl erefl.
+    { left. exists (Pair1 mx n' t)... }
+    { have[[nx stn]|vln]:=ihn erefl erefl.
+      { left. exists (Pair1 m' nx t)... }
+      { right... } } }
+  { move=>Γ Δ1 Δ2 Δ A B C m m' n n' s r t mrg tyC erm ihm ern ihn e1 e2; subst.
+    inv mrg. have[[mx stm]|vlm]:=ihm erefl erefl.
+    { left. exists (LetIn Box mx n')... }
+    { have[m1[m2 e]]:=
+        dyn_sig0_canonical
+          (era_dyn_type erm)
+          (convR _ _)
+          (era_dyn_val erm vlm). subst.
+      have[mx e]:=era_pair0_canonical erm. subst.
+      left. exists (n'.[Box,mx/])... } }
+  { move=>Γ Δ1 Δ2 Δ A B C m m' n n' s r1 r2 t mrg tyC erm ihm ern ihn e1 e2; subst.
+    inv mrg. have[[mx stm]|vlm]:=ihm erefl erefl.
+    { left. exists (LetIn Box mx n')... }
+    { have[m1[m2 e]]:=
+        dyn_sig1_canonical
+          (era_dyn_type erm)
+          (convR _ _)
+          (era_dyn_val erm vlm). subst.
+      have[mx[my e]]:=era_pair1_canonical erm. subst.
+      left. exists (n'.[my,mx/])... } }
+  { move=>Γ Δ A B m m' n n' t k erm ihm ern ihn e1 e2; subst. right... }
+  { move=>Γ Δ A B m m' t erm ihm e1 e2; subst.
+    have[[mx stm]|vlm]:=ihm erefl erefl.
+    { left. exists (Fst mx)... }
+    { have[m1[m2 e]]:=
+        dyn_with_canonical
+          (era_dyn_type erm)
+          (convR _ _)
+          (era_dyn_val erm vlm). subst.
+      have[mx[my e]]:=era_apair_canonical erm. subst.
+      left. exists mx... } }
+  { move=>Γ Δ A B m m' t erm ihm e1 e2; subst.
+    have[[mx stm]|vlm]:=ihm erefl erefl.
+    { left. exists (Snd mx)... }
+    { have[m1[m2 e]]:=
+        dyn_with_canonical
+          (era_dyn_type erm)
+          (convR _ _)
+          (era_dyn_val erm vlm). subst.
+      have[mx[my e]]:=era_apair_canonical erm. subst.
+      left. exists my... } }
   { move=>Γ Δ A B m m' s eq tym ihm tyB e1 e2; subst... }
 Qed.
