coq/era_subst.v
@@ -60,9 +60,6 @@ Lemma era_dyn_agree_subst Γ1 Γ2 Δ1 Δ2 σ1 σ2 :
   Γ1 ; Δ1 ⊢ σ1 ~ σ2 ⊣ Γ2 ; Δ2 -> Γ1 ; Δ1 ⊢ σ1 ⊣ Γ2 ; Δ2.
 Proof with eauto using dyn_agree_subst.
   elim=>{Γ1 Γ2 Δ1 Δ2 σ1 σ2}...
-  move=>Γ1 Γ2 σ1 σ2 Δ1 Δ2 Δa Δb n n' A s k mrg agr ih tyn.
-  apply: dyn_agree_subst_wk1...
-  apply: era_dyn_type...
 Qed.
 
 Lemma era_sta_agree_subst Γ1 Γ2 Δ1 Δ2 σ1 σ2 :
@@ -157,18 +154,12 @@ Proof with eauto 6 using merge, era_agree_subst, era_agree_subst_key.
     { have[Δa'[Δb'[mrg'[agra agrb]]]]:=ih _ _ H2.
       have[Δc[mrg1 mrg2]]:=merge_splitL mrg mrg'.
       exists Δc. exists Δb'.
-      repeat split...
-      apply: era_agree_subst_wk0...
-      apply: dyn_sta_type...
-      apply: era_dyn_type... }
+      repeat split... }
     { have[Δa'[Δb'[mrg'[agra agrb]]]]:=ih _ _ H2.
       have[Δc[mrg1 mrg2]]:=merge_splitR mrg mrg'.
       exists Δa'. exists Δc.
       repeat split...
-      exact: merge_sym.
-      apply: era_agree_subst_wk0...
-      apply: dyn_sta_type...
-      apply: era_dyn_type... } }
+      exact: merge_sym. } }
   { move=>Γ1 Δ1 σ1 σ2 Γ2 Δ2 A B s eq tyB1 tyB2 agr ih Δa Δb mrg. inv mrg.
     have[Δa'[Δb'[mrg'[agra agrb]]]]:=ih _ _ (merge_null H2).
     exists Δa'. exists Δb'... }
@@ -208,6 +199,44 @@ Proof with eauto using era_agree_subst, era_agree_subst_key, era_type.
     have{}ihm:=ihm _ _ _ _ agra.
     have{}ihn:=ihn _ _ _ _ agrb.
     apply: era_app1... }
+  { move=>Γ Δ A B m m' n t tyS tym ihm tyn Γ1 Δ1 σ1 σ2 agr. asimpl.
+    have{}ihS:=sta_substitution tyS (dyn_sta_agree_subst (era_dyn_agree_subst agr)).
+    have{}ihm:=ihm _ _ _ _ agr.
+    have{}ihn:=sta_substitution tyn (dyn_sta_agree_subst (era_dyn_agree_subst agr)).
+    apply: era_pair0...
+    asimpl. asimpl in ihn... }
+  { move=>Γ Δ1 Δ2 Δ A B m m' n n' t mrg tyS tym ihm tyn ihn Γ1 Δ0 σ1 σ2 agr. asimpl.
+    have[Δa[Δb[mrg0[agra agrb]]]]:=era_agree_subst_merge agr mrg.
+    have{}ihS:=sta_substitution tyS (dyn_sta_agree_subst (era_dyn_agree_subst agr)).
+    have{}ihm:=ihm _ _ _ _ agra.
+    have{}ihn:=ihn _ _ _ _ agrb.
+    apply: era_pair1...
+    asimpl. asimpl in ihn... }
+  { move=>Γ Δ1 Δ2 Δ A B C m m' n n' s r t mrg tyC tym ihm tyn ihn Γ1 Δ0 σ1 σ2 agr. asimpl.
+    have[Δa[Δb[mrg0[agra agrb]]]]:=era_agree_subst_merge agr mrg.
+    replace C.[m.[σ1] .: σ1] with C.[up σ1].[m.[σ1]/] by autosubst.
+    have wf:=sta_type_wf tyC. inv wf.
+    have wf:=dyn_type_wf (era_dyn_type tyn). inv wf. inv H4.
+    have{}ihC:=sta_substitution tyC
+      (sta_agree_subst_ty (dyn_sta_agree_subst (era_dyn_agree_subst agr)) H2).
+    have{}ihm:=ihm _ _ _ _ agra.
+    have{}ihn:=ihn _ _ _ _ (era_agree_subst_n (era_agree_subst_ty agrb H8) H5).
+    apply: era_letin0...
+    asimpl. asimpl in ihn... }
+  { move=>Γ Δ1 Δ2 Δ A B C m m' n n' s r1 r2 t mrg tyC tym ihm tyn ihn Γ1 Δ0 σ1 σ2 agr. asimpl.
+    have[Δa[Δb[mrg0[agra agrb]]]]:=era_agree_subst_merge agr mrg.
+    replace C.[m.[σ1] .: σ1] with C.[up σ1].[m.[σ1]/] by autosubst.
+    have wf:=sta_type_wf tyC. inv wf.
+    have wf:=dyn_type_wf (era_dyn_type tyn). inv wf. inv H4.
+    have{}ihC:=sta_substitution tyC
+      (sta_agree_subst_ty (dyn_sta_agree_subst (era_dyn_agree_subst agr)) H2).
+    have{}ihm:=ihm _ _ _ _ agra.
+    have{}ihn:=ihn _ _ _ _ (era_agree_subst_ty (era_agree_subst_ty agrb H8) H6).
+    apply: era_letin1...
+    asimpl. asimpl in ihn... }
+  { move=>Γ Δ A B m m' n n' t k tym ihm tyn ihn Γ1 Δ1 σ1 σ2 agr. asimpl. apply: era_apair... }
+  { move=>Γ Δ A B m m' t tym ihm Γ1 Δ1 σ1 σ2 agr. asimpl. apply: era_fst... }
+  { move=>Γ Δ A B m m' t tym ihm Γ1 Δ1 σ1 σ2 agr. asimpl. apply: era_snd... }
   { move=>Γ Δ A B m m' s eq tym ihm tyB Γ1 Δ1 σ1 σ2 agr.
     apply: era_conv.
     apply: sta_conv_subst...
