old/coq1/dyn_step.v
@@ -1,0 +1,30 @@
+From mathcomp Require Import ssreflect ssrbool eqtype ssrnat seq.
+From Coq Require Import ssrfun Classical Utf8.
+Require Export AutosubstSsr ARS tll_ast.
+
+Set Implicit Arguments.
+Unset Strict Implicit.
+Unset Printing Implicit Defensive.
+
+Inductive dyn_val : term -> Prop :=
+| dyn_val_var x : dyn_val (Var x)
+| dyn_val_lam0 A B s : dyn_val (Lam0 A B s)
+| dyn_val_lam1 A B s : dyn_val (Lam1 A B s).
+
+Reserved Notation "m ~>> n" (at level 30).
+Inductive dyn_step : term -> term -> Prop :=
+| dyn_appL m m' n :
+  m ~>> m' ->
+  App m n ~>> App m' n
+| dyn_appR m n n' :
+  n ~>> n' ->
+  App m n ~>> App m n'
+| dyn_beta0 A m n s :
+  App (Lam0 A m s) n ~>> m.[n/]
+| dyn_beta1 A m v s :
+  dyn_val v ->
+  App (Lam1 A m s) v ~>> m.[v/]
+where "m ~>> n" := (dyn_step m n).
+
+Notation dyn_red := (star dyn_step).
+Notation "m ~>>* n" := (dyn_red m n) (at level 30).
