old/coq1/era_sr.v
@@ -1,0 +1,79 @@
+From mathcomp Require Import ssreflect ssrbool eqtype ssrnat seq.
+From Coq Require Import ssrfun Classical Utf8.
+Require Export AutosubstSsr ARS era_inv.
+
+Set Implicit Arguments.
+Unset Strict Implicit.
+Unset Printing Implicit Defensive.
+
+Lemma era_dyn_val Γ Δ m m' A :
+  dyn_val m' -> Γ ; Δ ⊢ m ~ m' : A -> dyn_val m.
+Proof with eauto using dyn_val.
+  move=>vl. inv vl.
+  { move=>/era_var_form[x' e]; subst... }
+  { move=>/era_lam0_form[A'[m' e]]; subst... }
+  { move=>/era_lam1_form[A'[m' e]]; subst... }
+Qed.
+
+Theorem era_sr Γ Δ m m' n' A :
+  Γ ; Δ ⊢ m ~ m' : A -> m' ~>> n' ->
+  exists2 n, m ~>> n & Γ ; Δ ⊢ n ~ n' : A.
+Proof with eauto using dyn_step, era_type.
+  move=>er. elim: er n'=>{Γ Δ m m' A}.
+  { move=>Γ Δ x s A wf shs dhs n' st. inv st. }
+  { move=>Γ Δ A B m m' s k erm ihm n' st. inv st. }
+  { move=>Γ Δ A B m m' s t k erm ihm n' st. inv st. }
+  { move=>Γ Δ A B m m' n s erm ihm tyn n' st. inv st.
+    { have[x st tyx]:=ihm _ H2. exists (App x n)... }
+    { inv H2. }
+    { have[A'[m' e]]:=era_lam0_form erm.
+      subst. exists (m'.[n/])...
+      apply: era_subst0...
+      apply: era_lam0_inv... }
+    { have[A'[m' e]]:=era_lam1_form erm. subst.
+      have/dyn_sta_type ty:=era_dyn_type erm.
+      exfalso. apply: sta_lam1_pi0_false... } }
+  { move=>Γ Δ1 Δ2 Δ A B m m' n n' s mrg erm ihm ern ihn x st. inv st.
+    { have[x st tyx]:=ihm _ H2. exists (App x n)... }
+    { have[x st tyx]:=ihn _ H2. exists (App m x)...
+      have tym:=era_dyn_type erm.
+      have/dyn_sta_type tyn:=era_dyn_type ern.
+      have[_/sta_pi1_inv[r[tyB _]]]:=dyn_valid tym.
+      apply: era_conv.
+      apply: sta_conv_beta.
+      apply: conv1i.
+      apply: dyn_sta_step...
+      apply: era_app1...
+      have:=sta_subst tyB tyn.
+      asimpl... }
+    { have[A'[m' e]]:=era_lam0_form erm. subst.
+      have/dyn_sta_type ty:=era_dyn_type erm.
+      exfalso. apply: sta_lam0_pi1_false... }
+    { have[A'[m' e]]:=era_lam1_form erm.
+      subst. exists (m'.[n/])...
+      apply: dyn_beta1.
+      apply: era_dyn_val...
+      have{erm}[t erm]:=era_lam1_inv erm.
+      have wf:=dyn_type_wf (era_dyn_type erm). inv wf.
+      apply: era_subst1...
+      apply: dyn_val_key.
+      apply: era_dyn_type...
+      exact: H5.
+      apply: era_dyn_val... } }
+  { move=>Γ Δ A B m m' s eq tym ihm tyB n' st.
+    have[n st' tyn]:=ihm _ st.
+    exists n... }
+Qed.
+
+Corollary era_rd Γ Δ m m' n' A :
+  Γ ; Δ ⊢ m ~ m' : A -> m' ~>>* n' ->
+  exists2 n, m ~>>* n & Γ ; Δ ⊢ n ~ n' : A.
+Proof with eauto.
+  move=>ty rd. elim: rd Γ Δ m A ty=>{n'}...
+  move=>n n' rd ih st Γ Δ m A tym.
+  have[x rdx tyx]:=ih _ _ _ _ tym.
+  have[y sty tyy]:=era_sr tyx st.
+  exists y...
+  apply: star_trans...
+  apply: star1...
+Qed.
